src/C_strtoimax/AbstractSpec.v
@@ -147,10 +147,11 @@ Fixpoint string_at_address m s str dist : option (list byte) :=
           end
   end.
     
-Proposition asn_strtoimax_lim_fun_correct : forall s m str fin intp m' val,
+Proposition asn_strtoimax_lim_fun_correct : forall s m strp str fin intp m' val,
     asn_strtoimax_lim m str fin intp = Some {| return_type := ASN_STRTOX_OK ;
-                                             value := Some val ;
-                                             memory := m' |}
+                                               value := Some val ;
+                                               str_pointer := Some strp;
+                                               memory := m' |}
                                        <->
          addr_ge m str fin = Some false
          /\ string_at_address m nil str (distance str fin) = Some s
